share/everparse/tests/3d/specialize_test/src/main.c
@@ -147,21 +147,11 @@ BOOLEAN eq_p64_p32(P64 a, P32 b) {
 
 int test1(void) {
   A destA;
-  size_t a_out_pos = 0;
-  EVERPARSE_COPY_BUFFER_DESCR a_out_descr = {
-    .cb_base = (uint8_t*)&destA,
-    .cb_len = sizeof(destA),
-    .cb_pos = &a_out_pos
-  };
-  EVERPARSE_COPY_BUFFER_T a_out = &a_out_descr;
+  copy_buffer_t _cb_a_out = { .cb_base = (uint8_t*)&destA, .cb_len = sizeof(destA), .cb_pos = 0 };
+  EVERPARSE_COPY_BUFFER_T a_out = (EVERPARSE_COPY_BUFFER_T) &_cb_a_out;
   B64 destB;
-  size_t b_out_pos = 0;
-  EVERPARSE_COPY_BUFFER_DESCR b_out_descr = {
-    .cb_base = (uint8_t*)&destB,
-    .cb_len = sizeof(destB),
-    .cb_pos = &b_out_pos
-  };
-  EVERPARSE_COPY_BUFFER_T b_out = &b_out_descr;
+  copy_buffer_t _cb_b_out = { .cb_base = (uint8_t*)&destB, .cb_len = sizeof(destB), .cb_pos = 0 };
+  EVERPARSE_COPY_BUFFER_T b_out = (EVERPARSE_COPY_BUFFER_T) &_cb_b_out;
   if (SpecializeAbcCheckC(
       false, 
       a_out,
@@ -229,21 +219,11 @@ int test1(void) {
 
 int test2(void) {
   A destA = {0x00000000, 0x00000000};
-  size_t a_out_pos = 0;
-  EVERPARSE_COPY_BUFFER_DESCR a_out_descr = {
-    .cb_base = (uint8_t*)&destA,
-    .cb_len = sizeof(destA),
-    .cb_pos = &a_out_pos
-  };
-  EVERPARSE_COPY_BUFFER_T a_out = &a_out_descr;
+  copy_buffer_t _cb_a_out = { .cb_base = (uint8_t*)&destA, .cb_len = sizeof(destA), .cb_pos = 0 };
+  EVERPARSE_COPY_BUFFER_T a_out = (EVERPARSE_COPY_BUFFER_T) &_cb_a_out;
   B64 destB;
-  size_t b_out_pos = 0;
-  EVERPARSE_COPY_BUFFER_DESCR b_out_descr = {
-    .cb_base = (uint8_t*)&destB,
-    .cb_len = sizeof(destB),
-    .cb_pos = &b_out_pos
-  };
-  EVERPARSE_COPY_BUFFER_T b_out = &b_out_descr;
+  copy_buffer_t _cb_b_out = { .cb_base = (uint8_t*)&destB, .cb_len = sizeof(destB), .cb_pos = 0 };
+  EVERPARSE_COPY_BUFFER_T b_out = (EVERPARSE_COPY_BUFFER_T) &_cb_b_out;
   if (SpecializeAbcCheckC(
       false, 
       a_out,
