share/everparse/tests/3d/static/src/EverParseStream.c
@@ -1,4 +1,4 @@
-#include "EverParsePulseEndianness.h"
+#include "EverParseEndianness.h"
 #include "EverParseStream.h"
 #include <stdio.h>
 #include <stdlib.h>
